src/Init/Data/Array/Basic.lean
@@ -57,7 +57,7 @@ def singleton (v : α) : Array α :=
 def uget (a : @& Array α) (i : USize) (h : i.toNat < a.size) : α :=
   a[i.toNat]
 
-instance : GetElemBase (Array α) USize α fun xs i => i.toNat < xs.size where
+instance : GetElem (Array α) USize α fun xs i => i.toNat < xs.size where
   getElem xs i h := xs.uget i h
 
 def back [Inhabited α] (a : Array α) : α :=
