src/Init/Data/FloatArray/Basic.lean
@@ -55,10 +55,10 @@ def get? (ds : FloatArray) (i : Nat) : Option Float :=
   else
     none
 
-instance : GetElemBase FloatArray Nat Float fun xs i => i < xs.size where
+instance : GetElem FloatArray Nat Float fun xs i => i < xs.size where
   getElem xs i h := xs.get ⟨i, h⟩
 
-instance : GetElemBase FloatArray USize Float fun xs i => i.val < xs.size where
+instance : GetElem FloatArray USize Float fun xs i => i.val < xs.size where
   getElem xs i h := xs.uget i h
 
 @[extern "lean_float_array_uset"]
